examples/low-level/parsing/FStar.Format.fst
@@ -1,11 +1,11 @@
-module Format
+module FStar.Format
 
 open FStar.Ghost
 open FStar.UInt8
 open FStar.UInt32
 open FStar.Int.Cast
 open FStar.Seq
-open ImmBuffer
+open FStar.ImmBuffer
 
 type lsize = n:int{n = 1 \/ n = 2 \/ n = 3}
 type csize = n:t{v n = 1 \/ v n = 2 \/ v n = 3}
@@ -14,18 +14,25 @@ type csize = n:t{v n = 1 \/ v n = 2 \/ v n = 3}
 
 assume val aux_lemma_1: a:t -> b:t -> Lemma
   (requires (v a < pow2 8 /\ v b < pow2 8))
-  (ensures  (v a + (FStar.Mul (v b * pow2 8) % pow2 32) < pow2 16))
+  (ensures  (v a + (FStar.Mul.(v b * pow2 8) % pow2 32) < pow2 16))
 
 assume val aux_lemma_2: a:t -> b:t -> c:t -> Lemma
   (requires (v a < pow2 8 /\ v b < pow2 8))
-  (ensures  (v a + (FStar.Mul (v b * pow2 8) % pow2 32) 
-	         + (FStar.Mul (v c * pow2 16) % pow2 32) < pow2 24))
+  (ensures  (v a + (FStar.Mul.(v b * pow2 8) % pow2 32) 
+	         + (FStar.Mul.(v c * pow2 16) % pow2 32) < pow2 24))
+
+assume val pow2_increases_lemma:
+  (higher: nat) ->
+  (lower: nat) ->
+  Lemma
+  (requires (higher > lower))
+  (ensures (pow2 higher > pow2 lower))
 
 val read_length: b:buffer u8 -> n:csize{v n <= length b} -> Tot (l:UInt32.t{v l < pow2 24})
 let read_length b n =
   if n = 1ul then (
     let b0 = read b 0ul in
-    Math.Lib.pow2_increases_lemma 24 8;
+    pow2_increases_lemma 24 8;
     uint8_to_uint32 b0
   ) else if n = 2ul then (
     let b1 = read b 0ul in
@@ -33,8 +40,8 @@ let read_length b n =
     let b0 = uint8_to_uint32 b0 in
     let b1 = uint8_to_uint32 b1 in
     aux_lemma_1 b0 b1;
-    Math.Lib.pow2_increases_lemma 24 16;
-    Math.Lib.pow2_increases_lemma 32 24;
+    pow2_increases_lemma 24 16;
+    pow2_increases_lemma 32 24;
     b0 +^ (b1 <<^ 8ul)
   ) else (
     let b2 = read b 0ul in
@@ -44,7 +51,7 @@ let read_length b n =
     let b1 = uint8_to_uint32 b1 in
     let b2 = uint8_to_uint32 b2 in
     aux_lemma_2 b0 b1 b2;
-    Math.Lib.pow2_increases_lemma 32 24;
+    pow2_increases_lemma 32 24;
     b0 +^ (b1 <<^ 8ul) +^ (b2 <<^ 16ul)
   )
 
@@ -55,7 +62,7 @@ type lparser (#t:Type0) ($f:lserializer t) =
 
 type inverse (#t:Type0) ($f:lserializer t  ) ($g:lparser f) =
   (forall (x:t). g (f x) == Correct (x, lb_length (f x)))
-    /\ (forall (y:lbytes). Correct? (g y) ==>  (f (fst (Correct._0 (g y))) == y))
+    /\ (forall (y:lbytes). Correct? (g y) ==>  (f (fst (Correct?._0 (g y))) == y))
 
 noeq type lserializable (t:Type0) : Type0 =
   | VLSerializable: $f:lserializer t   -> $g:lparser f{inverse f g} -> lserializable t
@@ -69,7 +76,7 @@ assume HasSizeVLBytes: forall (n:lsize).
 val vlb_length: n:csize -> b:vlbytes (v n) -> Tot UInt32.t
 let vlb_length n b = read_length (sub b 0ul n) n
 
-#reset-options "--initial_fuel 0 --max_fuel 0 --z3timeout 5"
+#reset-options "--initial_fuel 0 --max_fuel 0"
 
 val read_length_lemma: #n:csize -> b:vlbytes (v n) -> j:UInt32.t{v j <= length b /\ v j >= v n} -> 
   Lemma (requires True)
@@ -86,7 +93,7 @@ let vlb_content (n:csize) (b:vlbytes (v n)) : Tot (buffer u8) =
 val vlserialize: n:csize -> Tot (lserializer (vlbytes (v n)))
 let vlserialize n = fun b -> (| read_length b n, b |)
 
-#reset-options "--initial_fuel 0 --max_fuel 0 --z3timeout 20"
+#reset-options "--initial_fuel 0 --max_fuel 0 --z3rlimit 20"
 
 let vlparse n : lparser (vlserialize n) = 
   fun (b:lbytes) ->
@@ -96,13 +103,13 @@ let vlparse n : lparser (vlserialize n) =
     else (
       let l = read_length bytes n in
       assume(v n < pow2 2);
-      Math.Lib.pow2_exp_lemma 2 24;
-      Math.Lib.pow2_increases_lemma 32 26;
+//      Math.Lib.pow2_exp_lemma 2 24;
+      pow2_increases_lemma 32 26;
       if len <^ n +^ l then Error "Wrong vlbytes format"
       else Correct (sub bytes 0ul (n +^ l), n +^ l)
     )
 
-#reset-options "--initial_fuel 0 --max_fuel 0 --z3timeout 5"
+#reset-options "--initial_fuel 0 --max_fuel 0 --z3rlimit 5"
 
 let rec valid_seq (#t:Type0) (ty:lserializable t) (b:lbytes) : Tot bool (decreases (v (lb_length b))) =  
   let len = lb_length b in
@@ -123,7 +130,7 @@ type vlbuffer (#t:Type0) (n:lsize) (ty:lserializable t) = b:buffer u8{
 val vlbuffer_serialize: #t:Type0 -> ty:lserializable t -> n:csize -> Tot (lserializer (vlbuffer (v n) ty))
 let vlbuffer_serialize #t ty n = fun b -> (| read_length b n, b |)
 
-#reset-options "--initial_fuel 0 --max_fuel 0 --z3timeout 20"
+#reset-options "--initial_fuel 0 --max_fuel 0 --z3rlimit 20"
 
 let vlbuffer_parse (#t:Type0) (ty:lserializable t) (n:csize) : lparser (vlbuffer_serialize ty n) 
   = fun b ->
@@ -133,8 +140,8 @@ let vlbuffer_parse (#t:Type0) (ty:lserializable t) (n:csize) : lparser (vlbuffer
     else (
       let l = read_length bytes n in
       assume (v n < pow2 2);
-      Math.Lib.pow2_exp_lemma 2 24;
-      Math.Lib.pow2_increases_lemma 32 26;
+//      Math.Lib.pow2_exp_lemma 2 24;
+      pow2_increases_lemma 32 26;
       if l +^ n >^ len then Error "Too short"
       else (
 	let b' = mk_lbytes (sub bytes n l) l in
@@ -143,7 +150,7 @@ let vlbuffer_parse (#t:Type0) (ty:lserializable t) (n:csize) : lparser (vlbuffer
       )
     )
 
-#reset-options "--initial_fuel 0 --max_fuel 0 --z3timeout 5"
+#reset-options "--initial_fuel 0 --max_fuel 0 --z3rlimit 5"
 
 noeq type key_share : Type0 = {
   ks_group_name: UInt16.t;
@@ -165,7 +172,7 @@ let vlserialize_key_share: lserializer key_share =
   fun ks -> (| 2ul +^ read_length ks.ks_public_key 2ul, 
     concat_buf #byte #u8 #byte #u8 (u16_to_buf ks.ks_group_name) (ks.ks_public_key) |)
 
-#reset-options "--initial_fuel 0 --max_fuel 0 --z3timeout 20"
+#reset-options "--initial_fuel 0 --max_fuel 0 --z3rlimit 20"
 
 val vlparse_key_share: p:lparser (vlserialize_key_share){inverse vlserialize_key_share p}
 let vlparse_key_share
